template-coq/theories/Environment.v
@@ -1,5 +1,5 @@
 (* Distributed under the terms of the MIT license. *)
-From MetaCoq.Template Require Import utils BasicAst.
+From MetaCoq.Template Require Import utils BasicAst utils.RTree.
 From MetaCoq.Template Require Import Universes.
 
 
@@ -120,26 +120,39 @@ Module Environment (T : Term).
 
   (** *** Environments *)
 
+  (* Recursive argument labels for representing the recursive structure of constructors of inductive types. *)
+  Inductive recarg := 
+    | Norec                 (* Non-recursive argument *)
+    | Mrec (i : inductive)  (* Recursive argument of type i *)
+    | Imbr (i : inductive). (* Recursive argument of "external" inductive type i, i.e. from another block of mutual inductives *)
+
+  (* the type used to represent the recursion structure of the arguments of constructors *)
+  Definition wf_paths := rtree recarg.
+
   (** See [one_inductive_body] from [declarations.ml]. *)
   Record one_inductive_body := {
     ind_name : ident;
     ind_type : term; (* Closed arity *)
     ind_kelim : sort_family; (* Top allowed elimination sort *)
-    ind_ctors : list (ident * term (* Under context of arities of the mutual inductive *)
+    ind_ctors : list (ident * term (* Under context of types of the mutual inductive (the inductives in the context still need to be given the parameters) *)
                       * nat (* arity, w/o lets, w/o parameters *));
     ind_projs : list (ident * term); (* names and types of projections, if any.
                                       Type under context of params and inductive object *)
-    ind_relevance : relevance (* relevance of the inductive definition *) }.
+    ind_relevance : relevance; (* relevance of the inductive definition *) 
+
+    ind_recargs : wf_paths (* recursive argument structure (inferred by the positivity checker) *)
+  }.
 
   Definition map_one_inductive_body npars arities f (n : nat) m :=
     match m with
-    | Build_one_inductive_body ind_name ind_type ind_kelim ind_ctors ind_projs ind_relevance =>
+    | Build_one_inductive_body ind_name ind_type ind_kelim ind_ctors ind_projs ind_relevance ind_recargs =>
       Build_one_inductive_body ind_name
                                (f 0 ind_type)
                                ind_kelim
                                (map (on_pi2 (f arities)) ind_ctors)
                                (map (on_snd (f (S npars))) ind_projs)
                                ind_relevance
+                               ind_recargs (* TODO: should be fine? *)
     end.
 
 
