template-coq/theories/Reflect.v
@@ -639,16 +639,37 @@ Proof.
   intros [] []; simpl; constructor; congruence.
 Defined.
 
+Require Import utils.RTree. 
+Instance reflect_rtree (X : Type) (H: ReflectEq X): ReflectEq (rtree X).
+Proof. 
+  refine {| eqb := rtree_eqb eqb |}.  
+  intros [] []; unfold rtree_eqb; simpl. 
+  (* TODO *)
+Admitted. 
+
+Definition eqb_recarg (x y : recarg) := 
+  match x, y with 
+  | Norec, Norec => true
+  | Mrec i, Mrec i' => eqb i i'
+  | Imbr i, Imbr i' => eqb i i'
+  | _, _ => false
+  end.
+Instance reflect_recarg : ReflectEq recarg. 
+Proof. 
+  refine {| eqb := eqb_recarg |}. 
+  intros [] []; unfold eqb_recarg; finish_reflect. 
+Defined.
+
 Definition eqb_one_inductive_body (x y : one_inductive_body) :=
-  let (n, t, k, c, p, r) := x in
-  let (n', t', k', c', p', r') := y in
-  eqb n n' && eqb t t' && eqb k k' && eqb c c' && eqb p p' && eqb r r'.
+  let (n, t, k, c, p, r, w) := x in
+  let (n', t', k', c', p', r', w') := y in
+  eqb n n' && eqb t t' && eqb k k' && eqb c c' && eqb p p' && eqb r r' && eqb w w'.
 
 Instance reflect_one_inductive_body : ReflectEq one_inductive_body.
 Proof.
   refine {| eqb := eqb_one_inductive_body |}.
   intros [] [].
-  unfold eqb_one_inductive_body; finish_reflect.
+  unfold eqb_one_inductive_body. finish_reflect.
 Defined.
 
 Definition eqb_Variance x y :=
